Added big step semantics. What do we do with pairs?

simple/simple.v
@@ -7,9 +7,11 @@ Notation "α ↪ β" := (link α β) (at level 90).
 Parameter weaken : forall {α β}, α↪β -> name β.
 Coercion weaken : link >-> name.
 Parameter import : forall {α β}, α↪β -> name α -> name β.
-Parameter next' : forall a, {b:world & a↪b}.
-Definition next a : {b:world & a↪b} := existT _ (projT1 (next' a)) (projT2 (next' a)).
+Parameter next' : forall α, {β:world & α↪β}.
+Definition next α : {β:world & α↪β} := existT _ (projT1 (next' α)) (projT2 (next' α)).
+Definition next_name α := projT2 (next' α).
 Parameter export : forall {α β} (y:α↪β) (n:name β), name α + unit.
+Axiom empty_is_empty : name ∅ -> False.
 
 Definition maybe {A C} (f:A -> C) (c:C) (x:A + unit) : C :=
 match x with
@@ -28,24 +30,33 @@ Inductive tp :=
 Set Implicit Arguments.
 Inductive exp (α:world) : Set :=
 | tt : exp α
+| var : name α -> exp α
 | lam : forall β, α↪β -> tp -> exp β -> exp α
 | app : exp α -> exp α -> exp α
 | fst : exp α -> exp α
 | snd : exp α -> exp α
 | pair : exp α -> exp α -> exp α.
 Implicit Arguments tt [α].
+Coercion var : name >-> exp.
 
-Definition ctx γ := name γ -> tp.
+Definition tp_ctx γ := name γ -> tp.
 
+Definition cdot {A} : name ∅ -> A :=
+fun n => match (empty_is_empty n) with end.
+Notation "·" := cdot.
 Notation "Γ ,, ( x , T )" := ((maybe Γ T) ○ (export x)) (at level 90).
 
 Reserved Notation "Γ ⊢ E ⇐ T" (at level 90).
 
-Inductive of {γ} (Γ:ctx γ) : exp γ -> tp -> Prop :=
+Inductive of {γ} (Γ:tp_ctx γ) : exp γ -> tp -> Prop :=
 | tt_of : Γ ⊢ tt ⇐ one
+| var_of : forall x T,
+          Γ x = T
+        (*===============================*) ->
+          Γ ⊢ x ⇐ T
 | lam_of : forall γ' (x:γ↪γ') T S M,
           Γ,,(x,T) ⊢ M ⇐ S
-        (*============================== *) ->
+        (*===============================*) ->
           Γ ⊢ lam x T M ⇐ arrow T S
 | app_of : forall T S M N,
           Γ ⊢ M ⇐ arrow T S ->
@@ -66,4 +77,68 @@ Inductive of {γ} (Γ:ctx γ) : exp γ -> tp -> Prop :=
         (*===============================*) ->
           Γ ⊢ pair M N ⇐ prod T S
 where "Γ ⊢ E ⇐ T" := (@of _ Γ E T).
+
+Inductive closure : Set :=
+| clos : forall γ, exp γ -> (name γ -> closure) -> closure.
+Definition env γ := name γ -> closure.
+Notation "E [ ρ ]" := (clos E ρ) (at level 80).
+
+Reserved Notation "C ∷ T" (at level 90).
+Inductive closure_of : closure -> tp -> Prop :=
+| clos_of : forall γ (M:exp γ) (Γ:tp_ctx γ) (ρ:env γ) T,
+            (forall x, (ρ x) ∷ (Γ x)) ->
+            Γ ⊢ M ⇐ T ->
+          (*==============================*)
+            M [ρ] ∷ T
+where "C ∷ T" := (closure_of C T).
+
+Inductive val : closure -> Prop :=
+ | fn_val : forall γ γ' (x:γ↪γ') M T ρ,
+      env_val ρ -> val ((lam x T M)[ρ])
+ | tt_val : forall γ (ρ:env γ),
+      env_val ρ -> val (tt[ρ])
+ | pair_val : forall γ (ρ:env γ) M N,
+      env_val ρ -> val (M[ρ]) -> val (N[ρ])
+   -> val ((pair M N)[ρ])
+with env_val : forall {γ}, env γ -> Prop :=
+ | env_val_nil : env_val ·
+ | env_val_cons : forall γ (ρ:env γ) γ' (x:γ↪γ') V,
+      val V -> env_val (ρ,,(x,V)).
+
+Reserved Notation "C ⇓ V" (at level 90).
+Definition X := next_name ∅.
+Definition Y := next_name (projT1 (next' ∅)).
+Inductive eval : closure -> closure -> Prop :=
+| val_eval : forall V,
+          val V
+        (*======*) ->
+          V ⇓ V 
+| var_eval : forall γ (ρ:env γ) x V,
+          ρ x = V
+        (*=========*) ->
+          x[ρ] ⇓ V
+| app_eval : forall γ γ' γ'' (ρ:env γ) ρ' (x:γ'↪γ'') T M N M' V1 V2,
+          M[ρ] ⇓ (lam x T M')[ρ'] ->
+          N[ρ] ⇓ V1 ->
+          M'[ρ',,(x,V1)] ⇓ V2
+        (*========================*) ->
+          (app M N)[ρ] ⇓ V2  
+| fst_eval : forall γ γ' (ρ:env γ) (ρ':env γ') M U V,
+          M[ρ] ⇓ (pair U V)[ρ']
+        (*========================*) ->
+          (fst M)[ρ] ⇓ U[ρ']
+| snd_eval : forall γ γ' (ρ:env γ) (ρ':env γ') M U V,
+          M[ρ] ⇓ (pair U V)[ρ']
+        (*========================*) ->
+          (snd M)[ρ] ⇓ V[ρ']
+(* | pair_eval : forall γ γ' (ρ:env γ) (ρ':env γ') M N V1 V2,
+          M[ρ] ⇓ V1 ->
+          N[ρ] ⇓ V2 ->
+          (pair M N)[ρ] ⇓ (pair (import Y X) Y)[·,,(X,V1),,(Y,V2)]*)
+where "C ⇓ V" := (eval C V).
+
+Hint Constructors eval val.
+Lemma eval_val V : val V -> eval V V.
+induction 1; eauto.
+Qed.
 
